\documentclass{beamer}
\usepackage[most]{tcolorbox}
\usepackage{fontawesome5}
\usepackage{hyperref}  
\tcbuselibrary{skins, breakable, listings}

\title{Mathmatical Foundations for Deep Generative Models}
\author{Michael Jin}
\date{\today}
\institute{
  \small
  \faGithub\ \href{https://github.com/Michael-J1n/Mathematical-Foundation-for-Deep-Generative-Models}{\texttt{Michael-J1n}} \\[1ex]
}

\begin{document}

\frame{\titlepage}

\begin{frame}[t]
\frametitle{Ultimate Goal}
\begin{tcolorbox}[colback=blue!1!white,
                  colframe=blue!75!black]
$$\theta^*=\arg\min_\theta\mathcal{D}\left(p_{\text{data}}(x) \mid
\mid p_\theta\right)$$
\end{tcolorbox}
\vspace{2em}
\begin{itemize}
\item $p_\theta$: model parameterized by $\theta$; e.g., neural network in DGM
    \begin{itemize}
        \item Q: what does the model stand for?
        \item A: \textbf{probability density function} for data distribution
    \end{itemize}
\item $p_\text{data}$: real data distribution in terms of p.d.f.
    \begin{itemize}
        \item Q: do we really have?
        \item A: not really
    \end{itemize}
\item $\mathcal{D}$: a measure of `distance'
\end{itemize}
\end{frame}

\begin{frame}[t]
\frametitle{Discrete v.s. Continuous}
Given sample data: $$A=\{x^1,x^2,\dots, x^N\},\quad x^i\in\mathbb{R}^d,\quad x^i\overset{\text{i.i.d.}}\sim p_{\text{data}}(x)$$ we can define the empirical distribution for estimating real distribution as:
\begin{tcolorbox}[colback=blue!1!white,
                  colframe=blue!75!black]
\[\displaystyle p_N(x)=\frac{1}{N}\sum_{i = 1}^N \mathbf{1}_{x^{i}\in A}=\frac{1}{N}\sum_{i = 1}^N \delta(x-x^{i})\]
\end{tcolorbox}

\begin{itemize}
    \item Probability mass function: $\displaystyle\int p_N(x)\text{d}x=\frac{1}{N}\sum_{i=1}^N\int \delta(x-x^i)\text{d}x=1$
    \item On expectation: $\displaystyle\mathbb{E}_{x\sim p_{N}(x)}[f(x)]=\sum_{i=1}^Nf(x^i)$
\end{itemize}
\end{frame}

\begin{frame}[t]
\frametitle{Measure divergence}
By information theory, optimal bit size for $x$ is $I(x)=-\log p(x)$. Hence we can define
\begin{itemize}
\item Information entropy for $p$: $$H(p)=\mathbb{E}_{x\sim p}[-\log p(x)]=-\int p(x)\log q(x)\text{d}x$$
\item Cross entropy if use $q$ to encode $p$:
$$H(p, q)=-\int p(x)\log q(x)\text{d}x$$
\end{itemize}
So how many bits are wasted if we use $q$ to encode $p$?
\begin{tcolorbox}[colback=blue!1!white,
                  colframe=blue!75!black]
$$\mathrm{D_{KL}}(p\mid\mid q)=H(p,q)-H(p)=\int p(x)\log\frac{p(x)}{q(x)}\text{d}x$$
\end{tcolorbox}
\end{frame}

\begin{frame}[t]
\frametitle{Lower Bound}
\begin{align*}
\mathrm{D_{KL}}(p\mid\mid q)&=\int p(x)\log\frac{p(x)}{q(x)}\text{d}x\\
&=-\int p(x)\log\frac{q(x)}{p(x)}\text{d}x\\
&\ge -\log\int p(x)\frac{q(x)}{p(x)}\text{d}x\\
&=-\log\int q(x)\text{d}x=-\log(1)=0
\end{align*}
\vspace{1em}
What about upper bound?\\
\quad \quad Consider for some $x$, $q(x)=0$; then $|\mathrm{D_{KL}}|\longrightarrow\infty$\\
\quad \quad Problem: Exploding Gradients
\end{frame}

\begin{frame}[t]
\frametitle{Solution}
We can measure the distance to average distribution instead.
Let $m(x)=\frac{1}{2}[p(x)+q(x)]$, then we define
\begin{tcolorbox}[colback=blue!1!white,
                  colframe=blue!75!black]
$$\mathrm{D_{JS}}(p\mid\mid q)=\frac{1}{2}\mathrm{D_{KL}}(p\mid\mid m)+\frac{1}{2}\mathrm{D_{KL}}(q\mid\mid m)
$$
\end{tcolorbox}
\begin{itemize}
    \item $\mathrm{D_{JS}}(p\mid\mid q)=\mathrm{D_{JS}}(q\mid\mid p)$
    \item Lower bound: $\mathrm{D_{JS}}\ge 0$ since $\mathrm{D_{KL}}\ge 0$
    \item Upper bound:
\end{itemize}
\end{frame}

\begin{frame}[t]
\frametitle{Upper Bound}
\begin{align*}
    \mathrm{D_{KL}}(p\mid\mid m)&=\int p(x)\log\frac{p(x)}{m(x)}\text{d}x\\
    &=\int p(x)\log\frac{p(x)}{\frac{1}{2}[p(x)+q(x)]}\text{d}x\\
    &\le \int p(x)\log \frac{2}{1+\frac{q(x)}{p(x)}}\text{d}x\\
    &\le \log{2}\int p(x)\text{d}x=\log{2}
\end{align*}
Therefore,
\begin{align*}
    \mathrm{D_{JS}}(p\mid\mid q)&=\frac{1}{2}\mathrm{D_{KL}}(p\mid\mid m)+\frac{1}{2}\mathrm{D_{KL}}(q\mid\mid m)\\
    &\le \frac{1}{2}\cdot 2\log2=\log2
\end{align*}
\end{frame}

\begin{frame}[t]
\frametitle{MLE}
Back to $A=\{x^i\}_{i=1}^N$, their joint probability for appearing in $p_\theta$:\\
$$
p_\theta(x^1,x^2,\dots, x^N)=\prod_{i=1}^Np_\theta(x^i)
$$
We want to maximize this probability, so
\begin{align*}
\theta^*&=\arg\max_\theta\prod_{i=1}^N p_\theta(x^i)\\
&=\arg\max_\theta\sum_{i=1}^N\log p_\theta(x^i)\\
&=\arg\max_\theta\mathbb{E}_{x\sim p_N}[\log p_\theta(x)]
\end{align*}

\begin{tcolorbox}[colback=blue!1!white,
                  colframe=blue!75!black]
$$
\hat\theta_{\text{MLE}}=\arg\max_\theta \mathbb{E}\left[\log p_\theta(x)\right]
$$
\end{tcolorbox}
\end{frame}

\begin{frame}[t]
\frametitle{MLE \& KLD}
\begin{align*}
    \mathrm{D_{KL}}(p_N\mid\mid p_\theta)&=\sum _{i=1}^Np_{N}\log\frac{p_N(x)}{p_\theta(x)}\\
    &=\sum_{i=1}^N p_N\log p_N(x)-\sum_{i=1}^N p_N(x)\log p_\theta(x)\\
    &=H(p_N)-\sum_{i=1}^N p_N(x)\log p_\theta(x)
\end{align*}
\end{frame}

\begin{frame}[t]
Therefore,
\begin{align*}
    \theta^*&=\arg\min_\theta\mathrm{D_{KL}}(p_{\text{data}}\mid\mid p_\theta)\\
    &=\arg\min_\theta \left[H(p_N)-\sum_{i=1}^N p_N(x)\log p_\theta(x)\right]\\
    &=\arg\max_\theta \sum_{i=1}^Np_N(x)\log p_\theta(x)\\
    &=\arg\max_\theta \mathbb{E}_{x\sim p_N(x)}[\log p_\theta(x)]
\end{align*}
\vspace{2em}
\begin{tcolorbox}[colback=blue!1!white,
                  colframe=blue!75!black]
$$
\hat\theta_\text{MLE}=\hat\theta_{\mathrm{D_{KL}}}
$$
\end{tcolorbox}
\end{frame}

\begin{frame}[t]
\frametitle{Next Step}
Here we finish some basic knowledge check. Back to the first slide, how can we build the model of $p_\theta(x)$?
Some known approaches:
\begin{itemize}
    \item Explicitly write down $p_\theta(x)$
    \item Implicitly get $p_\theta(x)$: use latent space
    \item learn a function about $p_\theta(x)$
\end{itemize}
\end{frame}

\begin{frame}[t]
\frametitle{Autoregressive}
Write $x=(x_1,x_2,\dots,x_d)\in\mathbb{R}^d$, then
$$
p(x)=p(x_1)\cdot p(x_2\mid x_1)\cdot p(x_3\mid x_1, x_2)\cdots p(x_d\mid x_{<d})
$$
That is,
\begin{tcolorbox}[colback=blue!1!white,
                  colframe=blue!75!black]
$$
p(x)=\prod_{t=1}^d p_\theta(x_t\mid x_{<t})
$$
\end{tcolorbox}
Hence,
\begin{align*}
    \theta^*&=\arg\max_\theta\sum_{i=1}^N\log p_\theta(x^i)\\
    &=\arg\max_\theta\sum_{i=1}^N\sum_{t=1}^T\log p_\theta(x_t^i\mid x_{<t}^i)
\end{align*}
\end{frame}

\begin{frame}[t]
\frametitle{Normalizing Flow (1)}
Introduce a simple distribution $z\sim p_Z(z)$ in the latent space $\mathbb{R}^d$.
Assume there exist a bijective function $f_\theta: z\longrightarrow x$ such that $f_{\theta}{_\#}p_Z=p_X$ (push-forward measure).

\vspace{2em}
By change of variable:
$$
\text{d}x=\left|\det\frac{\partial f}{\partial x}\right|\text{d}z :=\left|J_f(z)\text{d}z \right|
$$
and the probability conservation, we have:
\begin{align*}
p_X(x)\text{d}x&=p_Z(z)\text{d}z\\
&=p_Z(z)\left|\det \frac{\partial f}{\partial z}\right|^{-1}\text{d}x\quad\tag{*}
\end{align*}
\end{frame}

\begin{frame}[t]
\frametitle{Normalizing Flow (2)}
Recall that we have $(f^{-1}\circ f)(z)=I_d(z)$ for $\forall z\sim p_Z(z)$, so by chain rule,
$$
\frac{\partial f^{-1}}{\partial x}\cdot\frac{\partial f}{\partial z}=I_d
\Rightarrow \left(\frac{\partial f}{\partial z}\right)^{-1}=\frac{\partial f^{-1}}{\partial x}
$$
Hence $(*)\Longleftrightarrow$
$$p_X(x)=p_Z(z)\left|\det \frac{\partial f_\theta^{-1}}{\partial x}\right|$$
Or,
\begin{tcolorbox}[colback=blue!1!white,
                  colframe=blue!75!black]
$$p_\theta(x)=p_Z(f_\theta^{-1}(x))\left|\det \frac{\partial f_\theta^{-1}}{\partial x}\right|$$
\end{tcolorbox}
\end{frame}

\begin{frame}[t]
\frametitle{Normalizing Flow (3)}
And it follows that
\begin{align*}
\theta^*&=\arg\max_\theta\mathbb{E}_{x\sim p_N}\log p_\theta(x)\\
&=\arg\max_\theta \left[\log p_Z(f_\theta^{-1})+\log \left|\det \frac{\partial f_\theta^{-1}}{\partial x}\right|\right]
\end{align*}
\vspace{2em}
Base log-density + volume correction
\end{frame}

\begin{frame}[t]
\frametitle{GAN (1)}
\begin{itemize}
    \item In NF: $f$ has to be bijective, and requires a tractable Jacobian determinant
    vspace{1em}
    \item In GAN: Still assume simple distribution $z\sim p_Z(z)$ in the latent space $\mathbb{R}^k$.\\ Define generator $G_\theta: \mathbb{R}^k\to \mathbb{R}^d$ such that $x = G_\theta(z)$, where $G$ is not necessarily bijective.
    \begin{itemize}
        \item Problem: Unable to write down $\log p_\theta (x)$ \& perform MLE
        \vspace{1em}
        \item Solution: Add discriminator $D_\phi:\mathbb{R}^d\to [0,1]$ as supervising signal
    \end{itemize}
\end{itemize}

\vspace{1em}

Value function:
\begin{tcolorbox}[colback=blue!1!white,
                  colframe=blue!75!black]
$$
V(D, G)=\mathbb{E}_{x\sim p_N}[\log D(x)]+\mathbb{E}_{x\sim p_\theta}[\log(1-D(x))]
$$
\end{tcolorbox}

\end{frame}

\begin{frame}[t]
\frametitle{GAN (2)}
`Zero-sum game':
\begin{tcolorbox}[colback=blue!1!white,
                  colframe=blue!75!black]
$$
\min_G\max_DV(D, G)
$$
\end{tcolorbox}

Goal: given that $\phi$ is optimized, find an optimized $\theta$.\\
\vspace{1em}

1. Find the optimal $D_\phi$ given $G_\theta$ fixed:
$$
f(D)=p_N(x)\log(D(x))+p_\theta(x)\log(1-D(x))$$
$$
\Rightarrow \frac{\text{df}}{\text{d}D}=\frac{p_N(x)}{D(x)}-\frac{p_\theta(x)}{1-D(x)}:=0
$$
$$
\Rightarrow D^*(x)=\frac{p_N(x)}{p_N(x)+p_\theta(x)}
$$
\end{frame}

\begin{frame}[t]
\frametitle{GAN (3)}
2. Find the optimal $G_\theta$ given optimal $D_\phi$:

Denote $m(x)=\displaystyle\frac{1}{2}[p_N(x)+p_\theta(x)]$, then 
\begin{align*}
    V(D*, G)&=\mathbb{E}_{x\sim p_N}\left[\log\frac{p_N(x)}{2m(x)}\right]+\mathbb{E}_{x\sim p_\theta}\left[\log\frac{p_\theta(x)}{2m(x)}\right]\\
    &=2\left(\frac{1}{2}\mathbb{E}_{x\sim p_N}\left[\log\frac{p_N(x)}{m(x)}\right]+\frac{1}{2}\mathbb{E}_{x\sim p_\theta}\left[\log\frac{p_\theta(x)}{m(x)}\right]-\log2\right)\\
    &=2\mathrm{D_{JS}}(p_N\mid\mid p_\theta) - 2\log2
\end{align*}
Therefore,
\begin{tcolorbox}[colback=blue!1!white,
                  colframe=blue!75!black]
$$
\min_GV(D^*,G)\Longleftrightarrow\arg\min_\theta \mathrm{D_{JS}}(p_N\mid\mid p_\theta)
$$
\end{tcolorbox}

\end{frame}

\begin{frame}[t]
\frametitle{VAE (1)}
\begin{itemize}
    \item So far, latent to real is in point to point fashion
    \item What about point to distribution?
\end{itemize}
\vspace{1em}

Simple distribution $z\sim p_Z(z)$ in latent space $\mathbb{R}^k$, find its ouput in $p_N$ as a distribution / p.d.f.:
$p_\theta(x|z)$.
\vspace{1em}

Then we can model $p_\theta(x)$ using marginalization:
\begin{align*}
p_\theta(x)=\int p_\theta(x|z)p(z)\text{d}z\quad\tag{**}
\end{align*}
\begin{itemize}
    \item Problem: $z$ is continuous and in high-dimensional space, how to avoid integrate w.r.t. it?
    \item Solution: see the following trick about ELBO:
\end{itemize}
\end{frame}

\begin{frame}[t]
\frametitle{VAE (2)}
Introduce another distribution $q_\phi(z|x)$, and by $(**):$
\begin{align*}
    \log p_\theta(x)&=\log \int q_\phi(z|x)\frac{p_\theta(x,z)}{q_\phi(z|x)}\text{d}x\\
    &\ge\int q_\phi(z|x)\log \frac{p_\theta(x,z)}{q_\phi(z|x)}\text{d}x\\
    &=\mathbb{E}_{z\sim q_\phi(z|x)}\left[\log\frac{p_\theta(x|z)p(z)}{q_\phi(z|x)}\right]\\
    &:=\text{ELBO}(x)
\end{align*}
Where
$$
\text{ELBO}(x)=\mathbb{E}_{z\sim q_\phi(z|x)}[\log p_\theta(x|z)-(\log q_\phi(z|x)-\log p(z))] \Longrightarrow
$$
\begin{tcolorbox}[colback=blue!1!white,
                  colframe=blue!75!black]
$$
\text{ELBO}(x)=\mathbb{E}_{z\sim q_\phi(z|x)}[\log p_\theta(x|z)]-\mathrm{D_{KL}}(q_\phi(z|x)\mid\mid p_Z(z))
$$
\end{tcolorbox}
\end{frame}

\begin{frame}[t]
\frametitle{VAE (3)}
We want to maximize log-likelihood, so we should maximize the \textbf{ELBO}:
$$
\theta^*, \phi^*=\arg\max_{\theta, \phi}\mathbb{E}_{z\sim q_\phi(z|x)}[\log p_\theta(x|z)]-\mathrm{D_{KL}}(q_\phi(z|x)\mid\mid p_Z(z))
$$
\vspace{2em}
Base log-density + posterior correction
\end{frame}

\begin{frame}[t]
\frametitle{EBM (1)}
Still, we want to momdel a $p_\theta(x)$ such that it has MLE to $p_N(x)$. Lets borrow some ideas from physics. 
\vspace{1em}

Inspired by Boltzman Distribution $\displaystyle p_i=\frac{1}{Z}\exp(-\frac{\epsilon_i}{kT})$, we can model the p.d.f. of data as proportional to their energy $E(x)$ (lower energy means higher density):
\begin{tcolorbox}[colback=blue!1!white,
                  colframe=blue!75!black]
$$
p_\theta(x)=\frac{\exp(-E_\theta(x))}{Z(\theta)}
$$
\end{tcolorbox}
where $\displaystyle Z(\theta)=\int \exp(-E_\theta(x))\text{d}x$ is called the partition function.
\end{frame}

\begin{frame}[t]
\frametitle{EBM (2)}
If the data is in low dimension, we can design (or fit) $E_\theta(x)$ and calculate the partition function to get log-likelihood.
\vspace{1em}

For example, Hopfiled Network (which is the 2024 Nobel Prize for physics):
$$
E_\theta(x)=-\frac{1}{2}x^TW_\theta x+b_\theta^Tx
$$
Sampling from EBM: Inspired by Langevin Dynamics,
$$
\frac{\text{d}x}{\text{d}t}=-\nabla_xE_\theta(x)+\sqrt{2\beta^{-1}}\eta(t)
$$
we can make the sampling process like
$$
x_{k+1}=x_k-\frac{\epsilon}{2}\nabla_xE_\theta(x_k)+\sqrt{\epsilon}\eta_k
$$
from the SDE's Eulerâ€“Maruyama solution.
\end{frame}

\begin{frame}[t]
\frametitle{EBM (3)}
But if the data is in high dimension, the partition function is hard to compute.\\
Solution: we can directly learn $\nabla_xE_\theta(x)$, since it is the only parametrized term in the sampling process. Rather then know where is the destination, we can just learn where to go!

Therefore,
$$
\log p_\theta(x)=\log\left[\frac{\exp(-E_\theta(x))}{Z(\theta)}\right]=-E_\theta(x)-\log Z(\theta)
$$
becomes
$$
\nabla_x\log p_\theta(x)=\nabla_x[-E_\theta(x)]-\nabla_x[\log Z(\theta)]=-\nabla_x[-E_\theta(x)]
$$
and hence we can learn the score function
\begin{tcolorbox}[colback=blue!1!white,
                  colframe=blue!75!black]
$$
S_\theta(x)=\nabla_x\log p_\theta(x)
$$
\end{tcolorbox}
\end{frame}

\begin{frame}[t]
\frametitle{SBM (1)}
Recall that the score function is in fact the gradient field for probability distribution.\\
Before write down its detailed formulae, we need to first introduce the \textbf{Fisher Divergence}. It measures the difference of gradient fields for probability distributions:
$$
\mathrm{D_F}(p\mid\mid q)=\frac{1}{2}\int p(x)||\nabla_x\log p(x)-\nabla_x\log q(x)||^2\text{d}x
$$
So we can try to make the goal for SBM as following:
$$
\theta^*=\arg\min_\theta\mathbb{E}_{x\sim p_N}[||s_\theta(x)-\nabla_x\log p_N(x)||^2]
$$
but we cannot get the gradient for a discrete function $p_N(x)$.
\end{frame}

\begin{frame}[t]
\frametitle{SBM (2)}
Solution: lets go back to Fisher Divergence,
\begin{align*}
    \mathrm{D_F}(p\mid\mid q)&=\frac{1}{2}\mathbb{E}_{x\sim p}\left[||\nabla_x\log p(x)-\nabla_x\log q(x)||^2\right]\\
    &=\frac{1}{2}\mathbb{E}_{x\sim p}[||\nabla_x\log p(x)||^2-2\langle \nabla_x\log p(x), \nabla_x\log q(x)\rangle\\&\quad+||\nabla_x\log q(x)||^2 ]\tag{\#}
\end{align*}
where
\begin{align*}
&\mathbb{E}_{x\sim p}\langle \nabla_x\log p(x), \nabla_x\log q(x)\rangle\\&=\int p(x)[\nabla_x\log p(x)]^T\nabla_x\log q(x)\text{d}x\\
&=\int p(x)\left[\sum_i \nabla_x\log p(x_i)\nabla_x\log q(x_i)\right]\text{d}x\\
&=\sum_i\int p(x_i)\cdot \frac{\nabla_x p(x_i)}{p(x_i)}\nabla_x\log q(x_i)\text{d}x
\end{align*}
\end{frame}

\begin{frame}[t]
\frametitle{SBM (3)}
\begin{align*}
&=\sum_i\int \nabla_x\log q(x_i)\text{d}[p(x_i)]\\
&=\sum_i\left(\left[p(x_i)\nabla_x\log q(x_i)\right]_{\infty}^{\infty}-\int p(x_i)\nabla_x^2\log q(x_i)\text{d}x\right)\\
&=-\sum_i\int p(x_i)\nabla_x^2\log q(x_i)\text{d}x\\
&=-\int p(x)\left(\sum_i \nabla_x^2\log q(x_i)\right)\text{d}x\\
&=-\int p(x)\Delta_x \log q(x)\text{d}x\\
&=-\mathbb{E}_{x\sim p(x)}[\Delta_x \log q(x)]
\end{align*}
\end{frame}

\begin{frame}[t]
\frametitle{SBM (4)}
Then plug this back to $(\#):$
\begin{align*}
&\quad\mathrm{D_F}(p\mid\mid q)\\&=\mathbb{E}_{x\sim p}\left(\frac{1}{2}||\nabla_x\log p(x)||^2+2\Delta_x\log q(x)+\frac{1}{2}||\nabla_x\log q(x)||^2\right)
\end{align*}
Therefore,
\begin{align*}
&\mathrm{D_F}(p_N\mid\mid p_\theta)\\&=\mathbb{E}_{x\sim p_N(x)}\left(2\Delta_x\log p_\theta(x)+\frac{1}{2}||\nabla_x\log p_\theta(x)||^2\right)+C\\
&=\mathbb{E}_{x\sim p_N(x)}\left(2\nabla_x s_\theta(x)+\frac{1}{2}||s_\theta(x)||^2\right)+C
\end{align*}
And hence
\begin{tcolorbox}[colback=blue!1!white,
                  colframe=blue!75!black]
$$\theta^*=\arg\min_\theta \mathbb{E}_{x\sim p_N(x)}\left[2\nabla_x s_\theta(x)+\frac{1}{2}||s_\theta(x)||^2\right]$$
\end{tcolorbox}
\end{frame}

\begin{frame}[t]
\frametitle{DSM (1)}
Traditional score matching is uneasy \& costly to compute, so another approach is introduced: add noise.
\vspace{1em}

Let $x\sim p_N(x)$, we `smooth' this sample to a distribution: $q(\tilde{x}|x)\sim \mathcal{N}(\tilde{x};x,\sigma^2\mathrm{I})$. It can be seen as $\tilde{x}=x+\epsilon$, where $\epsilon$ is a noise.
Assume we have a $\tilde{x}$, we still need to let model learn `where to go', that is to trace along the gradient field for log-likelihood, i.e., the score function.
\vspace{1em}

We know by marginalization that
$$
p(\tilde{x})=\int p_N(x)q(\tilde{x}|x)\text{d}x=\mathbb{E}_{x\sim p_N(x)}[q(\tilde{x}|x)]
$$
Hence:
\end{frame}

\begin{frame}[t]
\frametitle{DSM (2)}
\begin{align*}
s(\tilde{x})&=\nabla_{\tilde{x}}\log p(\tilde{x})=\frac{1}{p(\tilde{x})}\nabla{_\tilde{x}}p(\tilde{x})
=\frac{1}{p(\tilde{x})}\nabla_{\tilde{x}} \int p_N(x)q(\tilde{x}|x)\text{d}x\\
&=\frac{1}{p(\tilde{x})}\int p_N(x)\nabla_{\tilde{x}}q(\tilde{x}|x)\text{d}x
=\int \frac{p_N(x)q(\tilde{x}|x)}{p(\tilde{x})}\nabla_{\tilde{x}}\log q(\tilde{x}|x)\text{d}x\\
&=\int p(x|\tilde{x})\nabla_{\tilde{x}}\log q(\tilde{x}|x)\text{d}x=\mathbb{E}_{x\sim p(x|\tilde{x})}[\nabla_{\tilde{x}}\log q(\tilde{x}|x)]
\end{align*}
Since $q$ is a normal distribution, $\displaystyle q(\tilde{x}|x)=k\exp\left(\frac{||\tilde{x}-x||^2}{-2\sigma^2}\right)$, so $\displaystyle\nabla{_\tilde{x}}\log q(\tilde{x}|x)=\frac{x-\tilde{x}}{\sigma^2}$. Therefore,
\begin{tcolorbox}[colback=blue!1!white,
                  colframe=blue!75!black]
$$
s(\tilde{x})=\frac{1}{\sigma^2}\mathbb{E}_{x\sim p(x|\tilde{x})}[x-\tilde{x}]
$$
\end{tcolorbox}
\end{frame}

\begin{frame}[t]
\frametitle{DSM (3)}
From their, we can then by linearity of expectation to get
$$
\mathbb{E}_{x\sim p(x|\tilde{x})}[x]=\tilde{x}+\sigma^2\nabla_{\tilde{x}}\log p(\tilde{x})
$$
which shows that the score function is the direction of denoising.
\vspace{1em}

For the LHS, we cannot directly get, but we can use a network $f_\theta$:
$\displaystyle s(\tilde{x})=\frac{f_\theta(\tilde{x})-\tilde{x}}{\sigma^2}$ to learn it, using simple MSE:
$$
\theta^*=\arg\min_\theta \mathbb{E}_{x\sim p_N(x),\tilde{x}\sim q({\tilde{x}}|x)}[||f_\theta({\tilde{x}})-x||^2]
$$

For sampling process ($x_T$ to $x_0$), still use Langevin Dynamics:
$$
x_{t-1}=x_{t}+\frac{\epsilon}{2\sigma^2}[f_\theta(x_t)-x_t]+\sqrt{\epsilon}\eta_t
$$
\end{frame}

\begin{frame}[t]
\frametitle{DSM (4)}
From DSM to DDPM: multi-step noise adding as a Markov process (which means there is a new parameter $t$ to control for time frame)
$$
q(x_t|x_{t-1})=\mathcal{N}(x_t;\sqrt{1-\beta_t}x_{t-1},\beta_t\mathrm{I})
$$
which can lead to the following closed form simply by adding multiple normal distributions:
$$
q(x_t|x_0)=\mathcal{N}(x_t;\sqrt{\bar{\alpha}_t}x_0,(1-\bar\alpha_t)\mathrm{I})
$$
which can also be written as 
\begin{tcolorbox}[colback=blue!1!white,
                  colframe=blue!75!black]
$$
x_t=\sqrt{\bar\alpha_t}x_0+\sqrt{1-\bar\alpha_t}\epsilon
$$
\end{tcolorbox}
Therefore,
$$
\nabla_{x_t}\log q(x_t|x_0)=-\frac{1}{1-\bar\alpha_t}(x_t-\sqrt{\bar\alpha_t}x_0)=
\frac{1}{\sqrt{1-\bar\alpha_t}}\epsilon
$$
\end{frame}

\begin{frame}[t]
\frametitle{DSM (5)}

We can use a function (network) parametrized by $\theta$, $s_\theta$, to learn for the score of the noise sample. Back to the original score fisher-divergence loss:
\begin{align*}
\theta^*&=\arg\min_\theta\mathbb{E}_{x_0\sim q(x_0), x_t\sim q(x_t|x_0)}[||s_\theta(x_t,t)-s(x_t,t)||^2]\\
&=\arg\min_\theta \mathbb{E}_{x_0\sim q(x_0), x_t\sim q(x_t|x_0)}[||s_\theta(x_t,t)+\frac{1}{\sqrt{1-\bar\alpha_t}}\epsilon||^2]\\
&=\arg\min_\theta \mathbb{E}_{x_0\sim q(x_0), x_t\sim q(x_t|x_0)}[||-\frac{1}{\sqrt{1-\bar\alpha_t}}\epsilon_\theta(x_t,t)+\frac{1}{\sqrt{1-\bar\alpha_t}}\epsilon||^2]
\end{align*}
\begin{tcolorbox}[colback=blue!1!white,
                  colframe=blue!75!black]
$$&=\arg\min_\theta \mathbb{E}[\epsilon-\epsilon_\theta(x_t,t)]$$
\end{tcolorbox}
Which shows that it is equivalent to construct a network for predicting noise!
\end{frame}

\begin{frame}[t]
\frametitle{What's more?}
If you think this is not enough, you can explore more on how differential equations work with generative models. In fact, diffusion process is closely related to Stochastic Differential Equations:
\vspace{1em}

The forward process (add noise) is
$$
\text{d}x=-\frac{1}{2}\beta_tx\text{d}t+\sqrt{\beta_t}\text{d}W
$$
where we call the coefficient to $\text{d}t$ the drift term $f(x,t)$, and $\text{d}W$ is a Brownian motion in $\mathbb{R}^d$, where its coefficient is the diffusion term $g(x,t)$.
Its corresponding reverse process (denoise) can be computed using Kologorov equations, and the result looks like
$$
\text{d}x=[-\frac{1}{2}\beta_tx-\beta_t\nabla_x\log p(x)]\text{d}t+\sqrt{\beta_t}\text{d}\tilde{W}
$$

\end{frame}

\end{document}
